src/Init/Data.lean
@@ -47,3 +47,4 @@ import Init.Data.Function
 import Init.Data.RArray
 import Init.Data.Vector
 import Init.Data.Iterators
+import Init.Data.Range.New.Nat
