src/Init/Data/Range.lean
@@ -8,4 +8,3 @@ module
 prelude
 import Init.Data.Range.Basic
 import Init.Data.Range.Lemmas
-import Init.Data.Range.New.Nat
