src/Init/Data/Range/New/Lemmas.lean
@@ -11,55 +11,121 @@ open Std.Iterators
 
 variable {shape : RangeShape} {α : Type u}
 
-private theorem toList_eq_toList_iterInternal [HasRange shape α] [UpwardEnumerable α]
-    [UpwardEnumerableRange shape α] [FinitelyEnumerableRange shape α]
-    [LawfulUpwardEnumerable α] [LawfulUpwardEnumerableRange shape α]
-    {r : PRange shape α} :
+private theorem toList_eq_toList_iterInternal [UpwardEnumerable α]
+    [UpwardEnumerableRange sl α] [SupportsUpperBound su α] [FinitelyEnumerableRange su α]
+    [LawfulUpwardEnumerable α]
+    {r : PRange ⟨sl, su⟩ α} :
     r.toList = r.iterInternal.toList := by
   rfl
 
--- observations:
--- would be nice to have non-dependent eq_match_step lemmas
--- need to support left-closed ranges as soon as any kind of range is supported
-theorem toList_eq_match [HasRange shape α] [UpwardEnumerable α]
-    [UpwardEnumerableRange shape α] [FinitelyEnumerableRange shape α]
-    [LawfulUpwardEnumerable α] [LawfulUpwardEnumerableRange shape α]
-    {r : PRange shape α} :
-    r.toList = match UpwardEnumerableRange.init r.lower with
+theorem toList_eq_match [UpwardEnumerable α]
+    [SupportsUpperBound su α] [FinitelyEnumerableRange su α]
+    [LawfulUpwardEnumerable α]
+    {it : Iter (α := Types.RangeIterator ⟨sl, su⟩ α) α} :
+    it.toList =  match it.internalState.next with
       | none => []
-      | some a => a ::  := by sorry
-
-theorem toList_eq_nil_iff [HasRange shape α] [UpwardEnumerable α]
-    [UpwardEnumerableRange shape α] [FinitelyEnumerableRange shape α]
-    [LawfulUpwardEnumerable α] [LawfulUpwardEnumerableRange shape α]
-    {r : PRange shape α} :
-    r.toList = [] ↔
-      ¬ (∃ a, UpwardEnumerableRange.init r.lower = some a ∧ HasRange.SatisfiesUpperBound r.upper a) := by
-  rw [toList_eq_toList_iterInternal, Iter.toList_eq_match_step, Types.RangeIterator.step_eq_step]
+      | some a => if SupportsUpperBound.IsSatisfied it.internalState.upperBound a then
+          a :: (⟨⟨UpwardEnumerable.succ? a, it.internalState.upperBound⟩⟩ : Iter (α := Types.RangeIterator ⟨sl, su⟩ α) α).toList
+        else
+          [] := by
+  rw [Iter.toList_eq_match_step, Types.RangeIterator.step_eq_step]
   simp only [Types.RangeIterator.step, PRange.iterInternal]
   split <;> rename_i heq <;> simp only [Subtype.mk.injEq] at heq
-  · split at heq
+  · split at heq <;> rename_i heq'
     · cases heq
-    · split at heq
-      · simp_all
-      · cases heq
-  · split at heq
-    · cases heq
-    · split at heq <;> cases heq
-  · split at heq
-    · simp_all
-    · rename_i heq'
-      split at heq
-      · cases heq
-      · simp_all
+    · split at heq <;> rename_i hs <;> cases heq
+      simp [heq', hs]
+  · split at heq <;> rename_i heq' <;> (try cases heq)
+    split at heq <;> cases heq
+  · split at heq <;> simp_all
 
-theorem mem_of_mem_toList [HasRange shape α] [UpwardEnumerable α]
-    [UpwardEnumerableRange shape α] [FinitelyEnumerableRange shape α]
-    [LawfulUpwardEnumerable α] [LawfulUpwardEnumerableRange shape α]
-    {r : PRange shape α}
-    {a : α} (h : a ∈ r.toList) :
-    a ∈ r := by
-  rw [toList_eq_toList_iterInternal] at h
-  replace h := Iter.isPlausibleIndirectOutput_of_mem_toList h
+theorem toList_eq_nil_iff [UpwardEnumerable α]
+    [SupportsUpperBound su α] [FinitelyEnumerableRange su α] [UpwardEnumerableRange sl α]
+    [LawfulUpwardEnumerable α]
+    {r : PRange ⟨sl, su⟩ α} :
+    r.toList = [] ↔
+      ¬ (∃ a, UpwardEnumerableRange.init r.lower = some a ∧ SupportsUpperBound.IsSatisfied r.upper a) := by
+  rw [toList_eq_toList_iterInternal] --, Iter.toList_eq_match_step, Types.RangeIterator.step_eq_step]
+  rw [toList_eq_match, PRange.iterInternal]
+  simp only
+  split <;> rename_i heq <;> simp [heq]
+
+theorem RangeIterator.mem_toList_iff_isPlausibleIndirectOutput
+    [UpwardEnumerable α] [UpwardEnumerableRange sl α]
+    [SupportsLowerBound sl α] [SupportsUpperBound su α]
+    [LawfulUpwardEnumerable α]
+    [LawfulUpwardEnumerableUpperBound su α] [LawfulUpwardEnumerableLowerBound sl α]
+    [FinitelyEnumerableRange su α]
+    {it : Iter (α := Types.RangeIterator ⟨sl, su⟩ α) α} :
+    out ∈ it.toList ↔ it.IsPlausibleIndirectOutput out := by
+  constructor
+  · apply Iter.isPlausibleIndirectOutput_of_mem_toList
+  · intro h
+    induction h
+    · rename_i it out h
+      rw [Types.RangeIterator.isPlausibleOutput_iff] at h
+      rw [toList_eq_match]
+      simp [h]
+    · rename_i it it' out h _ h'
+      rw [Types.RangeIterator.isPlausibleSuccessorOf_iff] at h
+      obtain ⟨a, ha⟩ := h
+      rw [toList_eq_match]
+      simp only [ha.1, ha.2.1, ha.2.2.1]
+      simp [← ha.2.2.2, h']
+
+theorem mem_toList_iff_mem [UpwardEnumerable α]
+    [SupportsUpperBound su α] [SupportsLowerBound sl α] [FinitelyEnumerableRange su α]
+    [UpwardEnumerableRange sl α] [LawfulUpwardEnumerable α]
+    [LawfulUpwardEnumerableLowerBound sl α] [LawfulUpwardEnumerableUpperBound su α]
+    {r : PRange ⟨sl, su⟩ α}
+    {a : α} : a ∈ r.toList ↔ a ∈ r := by
+  rw [toList_eq_toList_iterInternal, RangeIterator.mem_toList_iff_isPlausibleIndirectOutput,
+    RangeIterator.isPlausibleIndirectOutput_iff]
+
+theorem pairwise_upwardEnumerableLt [UpwardEnumerable α]
+    [SupportsUpperBound su α] [SupportsLowerBound sl α] [FinitelyEnumerableRange su α]
+    [UpwardEnumerableRange sl α] [LawfulUpwardEnumerable α]
+    [LawfulUpwardEnumerableLowerBound sl α] [LawfulUpwardEnumerableUpperBound su α]
+    {r : PRange ⟨sl, su⟩ α} :
+    r.toList.Pairwise (fun a b => UpwardEnumerable.lt a b) := by
+  rw [PRange.toList_eq_toList_iterInternal]
+  generalize r.iterInternal = it
+  induction it using Iter.inductSteps with | step it ihy ihs =>
+  rw [toList_eq_match]
+  repeat' split <;> (try exact .nil; done)
+  rename_i a _ _
+  apply List.Pairwise.cons
+  · intro a' ha
+    rw [RangeIterator.mem_toList_iff_isPlausibleIndirectOutput] at ha
+    replace ha := RangeIterator.upwardEnumerableLe_of_isPlausibleIndirectOutput ha
+    simp only at ha
+    have : UpwardEnumerable.lt a ha.choose := by
+      refine ⟨0, ?_⟩
+      simp only [LawfulUpwardEnumerable.succMany?_succ, LawfulUpwardEnumerable.succMany?_zero,
+        Option.bind_some]
+      exact ha.choose_spec.1
+    exact UpwardEnumerable.lt_of_lt_of_le this ha.choose_spec.2
+  · apply ihy (out := a)
+    simp_all [Types.RangeIterator.isPlausibleStep_iff, Types.RangeIterator.step]
+
+theorem forIn'_eq_forIn'_iterInternal [UpwardEnumerable α]
+    [SupportsUpperBound su α] [SupportsLowerBound sl α] [FinitelyEnumerableRange su α]
+    [UpwardEnumerableRange sl α] [LawfulUpwardEnumerable α]
+    [LawfulUpwardEnumerableLowerBound sl α] [LawfulUpwardEnumerableUpperBound su α]
+    {r : PRange ⟨sl, su⟩ α}
+    {γ : Type u} {init : γ} {m : Type u → Type w} [Monad m] {f : (a : α) → a ∈ r → γ → m (ForInStep γ)} :
+    ForIn'.forIn' r init f =
+      ForIn'.forIn' r.iterInternal init (fun a ha acc => f a (RangeIterator.isPlausibleIndirectOutput_iff.mp ha) acc) := by
+  rfl
+
+theorem forIn'_eq_forIn'_toList [UpwardEnumerable α]
+    [SupportsUpperBound su α] [SupportsLowerBound sl α] [FinitelyEnumerableRange su α]
+    [UpwardEnumerableRange sl α] [LawfulUpwardEnumerable α]
+    [LawfulUpwardEnumerableLowerBound sl α] [LawfulUpwardEnumerableUpperBound su α]
+    {r : PRange ⟨sl, su⟩ α}
+    {γ : Type u} {init : γ} {m : Type u → Type w} [Monad m] {f : (a : α) → a ∈ r → γ → m (ForInStep γ)} :
+    ForIn'.forIn' r init f =
+      ForIn'.forIn' r.toList init (fun a ha acc => f a (mem_toList_iff_mem.mp ha) acc) := by
+  simp only [forIn'_eq_forIn'_iterInternal, toList_eq_toList_iterInternal]
 
 end Std.PRange
